misc cleanup of ML bindings (for multihreading);

src/HOL/UNITY/Comp/Alloc.thy
@@ -30,7 +30,7 @@ constdefs
   client_map :: "'a clientState_d => clientState*'a"
     "client_map == funPair non_dummy dummy"
 
-  
+
 record allocState =
   allocGiv :: "nat => nat list"   --{*OUTPUT history: source of "giv" for i*}
   allocAsk :: "nat => nat list"   --{*INPUT: allocator's copy of "ask" for i*}
@@ -59,9 +59,9 @@ constdefs
   --{*spec (2)*}
   system_progress :: "'a systemState program set"
     "system_progress == INT i : lessThan Nclients.
-			INT h. 
-			  {s. h \<le> (ask o sub i o client)s} LeadsTo
-			  {s. h pfixLe (giv o sub i o client) s}"
+                        INT h.
+                          {s. h \<le> (ask o sub i o client)s} LeadsTo
+                          {s. h pfixLe (giv o sub i o client) s}"
 
   system_spec :: "'a systemState program set"
     "system_spec == system_safety Int system_progress"
@@ -81,9 +81,9 @@ constdefs
   --{*spec (5)*}
   client_progress :: "'a clientState_d program set"
     "client_progress ==
-	 Increasing giv  guarantees
-	 (INT h. {s. h \<le> giv s & h pfixGe ask s}
-		 LeadsTo {s. tokens h \<le> (tokens o rel) s})"
+         Increasing giv  guarantees
+         (INT h. {s. h \<le> giv s & h pfixGe ask s}
+                 LeadsTo {s. tokens h \<le> (tokens o rel) s})"
 
   --{*spec: preserves part*}
   client_preserves :: "'a clientState_d program set"
@@ -93,7 +93,7 @@ constdefs
   client_allowed_acts :: "'a clientState_d program set"
     "client_allowed_acts ==
        {F. AllowedActs F =
-	    insert Id (UNION (preserves (funPair rel ask)) Acts)}"
+            insert Id (UNION (preserves (funPair rel ask)) Acts)}"
 
   client_spec :: "'a clientState_d program set"
     "client_spec == client_increasing Int client_bounded Int client_progress
@@ -104,40 +104,40 @@ constdefs
   --{*spec (6)*}
   alloc_increasing :: "'a allocState_d program set"
     "alloc_increasing ==
-	 UNIV  guarantees
-	 (INT i : lessThan Nclients. Increasing (sub i o allocGiv))"
+         UNIV  guarantees
+         (INT i : lessThan Nclients. Increasing (sub i o allocGiv))"
 
   --{*spec (7)*}
   alloc_safety :: "'a allocState_d program set"
     "alloc_safety ==
-	 (INT i : lessThan Nclients. Increasing (sub i o allocRel))
+         (INT i : lessThan Nclients. Increasing (sub i o allocRel))
          guarantees
-	 Always {s. (SUM i: lessThan Nclients. (tokens o sub i o allocGiv)s)
+         Always {s. (SUM i: lessThan Nclients. (tokens o sub i o allocGiv)s)
          \<le> NbT + (SUM i: lessThan Nclients. (tokens o sub i o allocRel)s)}"
 
   --{*spec (8)*}
   alloc_progress :: "'a allocState_d program set"
     "alloc_progress ==
-	 (INT i : lessThan Nclients. Increasing (sub i o allocAsk) Int
-	                             Increasing (sub i o allocRel))
+         (INT i : lessThan Nclients. Increasing (sub i o allocAsk) Int
+                                     Increasing (sub i o allocRel))
          Int
          Always {s. ALL i<Nclients.
-		     ALL elt : set ((sub i o allocAsk) s). elt \<le> NbT}
+                     ALL elt : set ((sub i o allocAsk) s). elt \<le> NbT}
          Int
-         (INT i : lessThan Nclients. 
-	  INT h. {s. h \<le> (sub i o allocGiv)s & h pfixGe (sub i o allocAsk)s}
-		 LeadsTo
-	         {s. tokens h \<le> (tokens o sub i o allocRel)s})
+         (INT i : lessThan Nclients.
+          INT h. {s. h \<le> (sub i o allocGiv)s & h pfixGe (sub i o allocAsk)s}
+                 LeadsTo
+                 {s. tokens h \<le> (tokens o sub i o allocRel)s})
          guarantees
-	     (INT i : lessThan Nclients.
-	      INT h. {s. h \<le> (sub i o allocAsk) s}
-	             LeadsTo
-	             {s. h pfixLe (sub i o allocGiv) s})"
+             (INT i : lessThan Nclients.
+              INT h. {s. h \<le> (sub i o allocAsk) s}
+                     LeadsTo
+                     {s. h pfixLe (sub i o allocGiv) s})"
 
   (*NOTE: to follow the original paper, the formula above should have had
-	INT h. {s. h i \<le> (sub i o allocGiv)s & h i pfixGe (sub i o allocAsk)s}
-	       LeadsTo
-	       {s. tokens h i \<le> (tokens o sub i o allocRel)s})
+        INT h. {s. h i \<le> (sub i o allocGiv)s & h i pfixGe (sub i o allocAsk)s}
+               LeadsTo
+               {s. tokens h i \<le> (tokens o sub i o allocRel)s})
     thus h should have been a function variable.  However, only h i is ever
     looked at.*)
 
@@ -145,12 +145,12 @@ constdefs
   alloc_preserves :: "'a allocState_d program set"
     "alloc_preserves == preserves allocRel Int preserves allocAsk Int
                         preserves allocState_d.dummy"
-  
+
   --{*environmental constraints*}
   alloc_allowed_acts :: "'a allocState_d program set"
     "alloc_allowed_acts ==
        {F. AllowedActs F =
-	    insert Id (UNION (preserves allocGiv) Acts)}"
+            insert Id (UNION (preserves allocGiv) Acts)}"
 
   alloc_spec :: "'a allocState_d program set"
     "alloc_spec == alloc_increasing Int alloc_safety Int alloc_progress Int
@@ -161,22 +161,22 @@ constdefs
   --{*spec (9.1)*}
   network_ask :: "'a systemState program set"
     "network_ask == INT i : lessThan Nclients.
-			Increasing (ask o sub i o client)  guarantees
-			((sub i o allocAsk) Fols (ask o sub i o client))"
+                        Increasing (ask o sub i o client)  guarantees
+                        ((sub i o allocAsk) Fols (ask o sub i o client))"
 
   --{*spec (9.2)*}
   network_giv :: "'a systemState program set"
     "network_giv == INT i : lessThan Nclients.
-			Increasing (sub i o allocGiv)
-			guarantees
-			((giv o sub i o client) Fols (sub i o allocGiv))"
+                        Increasing (sub i o allocGiv)
+                        guarantees
+                        ((giv o sub i o client) Fols (sub i o allocGiv))"
 
   --{*spec (9.3)*}
   network_rel :: "'a systemState program set"
     "network_rel == INT i : lessThan Nclients.
-			Increasing (rel o sub i o client)
-			guarantees
-			((sub i o allocRel) Fols (rel o sub i o client))"
+                        Increasing (rel o sub i o client)
+                        guarantees
+                        ((sub i o allocRel) Fols (rel o sub i o client))"
 
   --{*spec: preserves part*}
   network_preserves :: "'a systemState program set"
@@ -184,15 +184,15 @@ constdefs
        preserves allocGiv  Int
        (INT i : lessThan Nclients. preserves (rel o sub i o client)  Int
                                    preserves (ask o sub i o client))"
-  
+
   --{*environmental constraints*}
   network_allowed_acts :: "'a systemState program set"
     "network_allowed_acts ==
        {F. AllowedActs F =
            insert Id
-	    (UNION (preserves allocRel Int
-		    (INT i: lessThan Nclients. preserves(giv o sub i o client)))
-		  Acts)}"
+            (UNION (preserves allocRel Int
+                    (INT i: lessThan Nclients. preserves(giv o sub i o client)))
+                  Acts)}"
 
   network_spec :: "'a systemState program set"
     "network_spec == network_ask Int network_giv Int
@@ -204,25 +204,25 @@ constdefs
   sysOfAlloc :: "((nat => clientState) * 'a) allocState_d => 'a systemState"
     "sysOfAlloc == %s. let (cl,xtr) = allocState_d.dummy s
                        in (| allocGiv = allocGiv s,
-			     allocAsk = allocAsk s,
-			     allocRel = allocRel s,
-			     client   = cl,
-			     dummy    = xtr|)"
+                             allocAsk = allocAsk s,
+                             allocRel = allocRel s,
+                             client   = cl,
+                             dummy    = xtr|)"
 
 
   sysOfClient :: "(nat => clientState) * 'a allocState_d => 'a systemState"
     "sysOfClient == %(cl,al). (| allocGiv = allocGiv al,
-			         allocAsk = allocAsk al,
-			         allocRel = allocRel al,
-			         client   = cl,
-			         systemState.dummy = allocState_d.dummy al|)"
+                                 allocAsk = allocAsk al,
+                                 allocRel = allocRel al,
+                                 client   = cl,
+                                 systemState.dummy = allocState_d.dummy al|)"
 
-consts 
+consts
     Alloc   :: "'a allocState_d program"
     Client  :: "'a clientState_d program"
     Network :: "'a systemState program"
     System  :: "'a systemState program"
-  
+
 axioms
     Alloc:   "Alloc   : alloc_spec"
     Client:  "Client  : client_spec"
@@ -232,12 +232,12 @@ defs
     System_def:
       "System == rename sysOfAlloc Alloc Join Network Join
                  (rename sysOfClient
-		  (plam x: lessThan Nclients. rename client_map Client))"
+                  (plam x: lessThan Nclients. rename client_map Client))"
 
 
 (**
 locale System =
-  fixes 
+  fixes
     Alloc   :: 'a allocState_d program
     Client  :: 'a clientState_d program
     Network :: 'a systemState program
@@ -255,7 +255,7 @@ locale System =
                  Network
                  Join
                  (rename sysOfClient
-		  (plam x: lessThan Nclients. rename client_map Client))"
+                  (plam x: lessThan Nclients. rename client_map Client))"
 **)
 
 (*Perhaps equalities.ML shouldn't add this in the first place!*)
@@ -287,62 +287,62 @@ lemmas [simp] =
   bij_image_Collect_eq
 
 ML {*
-local
-  val INT_D = thm "INT_D";
-in
 (*Splits up conjunctions & intersections: like CONJUNCTS in the HOL system*)
-fun list_of_Int th = 
+fun list_of_Int th =
     (list_of_Int (th RS conjunct1) @ list_of_Int (th RS conjunct2))
     handle THM _ => (list_of_Int (th RS IntD1) @ list_of_Int (th RS IntD2))
-    handle THM _ => (list_of_Int (th RS INT_D))
+    handle THM _ => (list_of_Int (th RS @{thm INT_D}))
     handle THM _ => (list_of_Int (th RS bspec))
     handle THM _ => [th];
-end;
 *}
 
 lemmas lessThanBspec = lessThan_iff [THEN iffD2, THEN [2] bspec]
 
-ML {*
-local
-  val lessThanBspec = thm "lessThanBspec"
+setup {*
+let
+  fun normalized th =
+    normalized (th RS spec
+      handle THM _ => th RS @{thm lessThanBspec}
+      handle THM _ => th RS bspec
+      handle THM _ => th RS (@{thm guarantees_INT_right_iff} RS iffD1))
+    handle THM _ => th;
 in
-fun normalize th = 
-     normalize (th RS spec
-		handle THM _ => th RS lessThanBspec
-		handle THM _ => th RS bspec
-		handle THM _ => th RS (guarantees_INT_right_iff RS iffD1))
-     handle THM _ => th
+  Attrib.add_attributes [("normalized", Attrib.no_args (Thm.rule_attribute (K normalized)), "")]
 end
 *}
 
 (*** bijectivity of sysOfAlloc [MUST BE AUTOMATED] ***)
 ML {*
-val record_auto_tac =
-  auto_tac (claset() addIs [ext] addSWrapper record_split_wrapper, 
-    simpset() addsimps [thm "sysOfAlloc_def", thm "sysOfClient_def",
-      thm "client_map_def", thm "non_dummy_def", thm "funPair_def", thm "o_apply", thm "Let_def"])
+fun record_auto_tac (cs, ss) =
+  auto_tac (cs addIs [ext] addSWrapper record_split_wrapper,
+    ss addsimps [@{thm sysOfAlloc_def}, @{thm sysOfClient_def},
+      @{thm client_map_def}, @{thm non_dummy_def}, @{thm funPair_def},
+      @{thm o_apply}, @{thm Let_def}])
 *}
 
+method_setup record_auto = {*
+  Method.ctxt_args (fn ctxt => Method.SIMPLE_METHOD (record_auto_tac (local_clasimpset_of ctxt)))
+*} ""
 
 lemma inj_sysOfAlloc [iff]: "inj sysOfAlloc"
   apply (unfold sysOfAlloc_def Let_def)
   apply (rule inj_onI)
-  apply (tactic record_auto_tac)
+  apply record_auto
   done
 
 text{*We need the inverse; also having it simplifies the proof of surjectivity*}
-lemma inv_sysOfAlloc_eq [simp]: "!!s. inv sysOfAlloc s =  
-             (| allocGiv = allocGiv s,    
-                allocAsk = allocAsk s,    
-                allocRel = allocRel s,    
+lemma inv_sysOfAlloc_eq [simp]: "!!s. inv sysOfAlloc s =
+             (| allocGiv = allocGiv s,
+                allocAsk = allocAsk s,
+                allocRel = allocRel s,
                 allocState_d.dummy = (client s, dummy s) |)"
   apply (rule inj_sysOfAlloc [THEN inv_f_eq])
-  apply (tactic record_auto_tac)
+  apply record_auto
   done
 
 lemma surj_sysOfAlloc [iff]: "surj sysOfAlloc"
   apply (simp add: surj_iff expand_fun_eq o_apply)
-  apply (tactic record_auto_tac)
+  apply record_auto
   done
 
 lemma bij_sysOfAlloc [iff]: "bij sysOfAlloc"
@@ -355,22 +355,22 @@ subsubsection{*bijectivity of @{term sysOfClient}*}
 lemma inj_sysOfClient [iff]: "inj sysOfClient"
   apply (unfold sysOfClient_def)
   apply (rule inj_onI)
-  apply (tactic record_auto_tac)
+  apply record_auto
   done
 
-lemma inv_sysOfClient_eq [simp]: "!!s. inv sysOfClient s =  
-             (client s,  
-              (| allocGiv = allocGiv s,  
-                 allocAsk = allocAsk s,  
-                 allocRel = allocRel s,  
+lemma inv_sysOfClient_eq [simp]: "!!s. inv sysOfClient s =
+             (client s,
+              (| allocGiv = allocGiv s,
+                 allocAsk = allocAsk s,
+                 allocRel = allocRel s,
                  allocState_d.dummy = systemState.dummy s|) )"
   apply (rule inj_sysOfClient [THEN inv_f_eq])
-  apply (tactic record_auto_tac)
+  apply record_auto
   done
 
 lemma surj_sysOfClient [iff]: "surj sysOfClient"
   apply (simp add: surj_iff expand_fun_eq o_apply)
-  apply (tactic record_auto_tac)
+  apply record_auto
   done
 
 lemma bij_sysOfClient [iff]: "bij sysOfClient"
@@ -382,19 +382,19 @@ subsubsection{*bijectivity of @{term client_map}*}
 
 lemma inj_client_map [iff]: "inj client_map"
   apply (unfold inj_on_def)
-  apply (tactic record_auto_tac)
+  apply record_auto
   done
 
-lemma inv_client_map_eq [simp]: "!!s. inv client_map s =  
-             (%(x,y).(|giv = giv x, ask = ask x, rel = rel x,  
+lemma inv_client_map_eq [simp]: "!!s. inv client_map s =
+             (%(x,y).(|giv = giv x, ask = ask x, rel = rel x,
                        clientState_d.dummy = y|)) s"
   apply (rule inj_client_map [THEN inv_f_eq])
-  apply (tactic record_auto_tac)
+  apply record_auto
   done
 
 lemma surj_client_map [iff]: "surj client_map"
   apply (simp add: surj_iff expand_fun_eq o_apply)
-  apply (tactic record_auto_tac)
+  apply record_auto
   done
 
 lemma bij_client_map [iff]: "bij client_map"
@@ -424,28 +424,28 @@ declare snd_o_client_map' [simp]
 subsection{*o-simprules for @{term sysOfAlloc} [MUST BE AUTOMATED]*}
 
 lemma client_o_sysOfAlloc: "client o sysOfAlloc = fst o allocState_d.dummy "
-  apply (tactic record_auto_tac)
+  apply record_auto
   done
 
 ML {* bind_thms ("client_o_sysOfAlloc'", make_o_equivs (thm "client_o_sysOfAlloc")) *}
 declare client_o_sysOfAlloc' [simp]
 
 lemma allocGiv_o_sysOfAlloc_eq: "allocGiv o sysOfAlloc = allocGiv"
-  apply (tactic record_auto_tac)
+  apply record_auto
   done
 
 ML {* bind_thms ("allocGiv_o_sysOfAlloc_eq'", make_o_equivs (thm "allocGiv_o_sysOfAlloc_eq")) *}
 declare allocGiv_o_sysOfAlloc_eq' [simp]
 
 lemma allocAsk_o_sysOfAlloc_eq: "allocAsk o sysOfAlloc = allocAsk"
-  apply (tactic record_auto_tac)
+  apply record_auto
   done
 
 ML {* bind_thms ("allocAsk_o_sysOfAlloc_eq'", make_o_equivs (thm "allocAsk_o_sysOfAlloc_eq")) *}
 declare allocAsk_o_sysOfAlloc_eq' [simp]
 
 lemma allocRel_o_sysOfAlloc_eq: "allocRel o sysOfAlloc = allocRel"
-  apply (tactic record_auto_tac)
+  apply record_auto
   done
 
 ML {* bind_thms ("allocRel_o_sysOfAlloc_eq'", make_o_equivs (thm "allocRel_o_sysOfAlloc_eq")) *}
@@ -455,28 +455,28 @@ declare allocRel_o_sysOfAlloc_eq' [simp]
 subsection{* o-simprules for @{term sysOfClient} [MUST BE AUTOMATED]*}
 
 lemma client_o_sysOfClient: "client o sysOfClient = fst"
-  apply (tactic record_auto_tac)
+  apply record_auto
   done
 
 ML {* bind_thms ("client_o_sysOfClient'", make_o_equivs (thm "client_o_sysOfClient")) *}
 declare client_o_sysOfClient' [simp]
 
 lemma allocGiv_o_sysOfClient_eq: "allocGiv o sysOfClient = allocGiv o snd "
-  apply (tactic record_auto_tac)
+  apply record_auto
   done
 
 ML {* bind_thms ("allocGiv_o_sysOfClient_eq'", make_o_equivs (thm "allocGiv_o_sysOfClient_eq")) *}
 declare allocGiv_o_sysOfClient_eq' [simp]
 
 lemma allocAsk_o_sysOfClient_eq: "allocAsk o sysOfClient = allocAsk o snd "
-  apply (tactic record_auto_tac)
+  apply record_auto
   done
 
 ML {* bind_thms ("allocAsk_o_sysOfClient_eq'", make_o_equivs (thm "allocAsk_o_sysOfClient_eq")) *}
 declare allocAsk_o_sysOfClient_eq' [simp]
 
 lemma allocRel_o_sysOfClient_eq: "allocRel o sysOfClient = allocRel o snd "
-  apply (tactic record_auto_tac)
+  apply record_auto
   done
 
 ML {* bind_thms ("allocRel_o_sysOfClient_eq'", make_o_equivs (thm "allocRel_o_sysOfClient_eq")) *}
@@ -503,7 +503,7 @@ lemma allocRel_o_inv_sysOfAlloc_eq: "allocRel o inv sysOfAlloc = allocRel"
 ML {* bind_thms ("allocRel_o_inv_sysOfAlloc_eq'", make_o_equivs (thm "allocRel_o_inv_sysOfAlloc_eq")) *}
 declare allocRel_o_inv_sysOfAlloc_eq' [simp]
 
-lemma rel_inv_client_map_drop_map: "(rel o inv client_map o drop_map i o inv sysOfClient) =  
+lemma rel_inv_client_map_drop_map: "(rel o inv client_map o drop_map i o inv sysOfClient) =
       rel o sub i o client"
   apply (simp add: o_def drop_map_def)
   done
@@ -511,7 +511,7 @@ lemma rel_inv_client_map_drop_map: "(rel o inv client_map o drop_map i o inv sys
 ML {* bind_thms ("rel_inv_client_map_drop_map'", make_o_equivs (thm "rel_inv_client_map_drop_map")) *}
 declare rel_inv_client_map_drop_map [simp]
 
-lemma ask_inv_client_map_drop_map: "(ask o inv client_map o drop_map i o inv sysOfClient) =  
+lemma ask_inv_client_map_drop_map: "(ask o inv client_map o drop_map i o inv sysOfClient) =
       ask o sub i o client"
   apply (simp add: o_def drop_map_def)
   done
@@ -519,17 +519,6 @@ lemma ask_inv_client_map_drop_map: "(ask o inv client_map o drop_map i o inv sys
 ML {* bind_thms ("ask_inv_client_map_drop_map'", make_o_equivs (thm "ask_inv_client_map_drop_map")) *}
 declare ask_inv_client_map_drop_map [simp]
 
-(**
-Open_locale "System"
-
-val Alloc = thm "Alloc";
-val Client = thm "Client";
-val Network = thm "Network";
-val System_def = thm "System_def";
-
-CANNOT use bind_thm: it puts the theorem into standard form, in effect
-  exporting it from the locale
-**)
 
 declare finite_lessThan [iff]
 
@@ -541,9 +530,9 @@ lemmas client_spec_simps =
 
 ML {*
 val [Client_Increasing_ask, Client_Increasing_rel,
-     Client_Bounded, Client_Progress, Client_AllowedActs, 
+     Client_Bounded, Client_Progress, Client_AllowedActs,
      Client_preserves_giv, Client_preserves_dummy] =
-        thm "Client" |> simplify (simpset() addsimps (thms "client_spec_simps") )
+        @{thm Client} |> simplify (@{simpset} addsimps @{thms client_spec_simps})
                |> list_of_Int;
 
 bind_thm ("Client_Increasing_ask", Client_Increasing_ask);
@@ -571,9 +560,9 @@ lemmas network_spec_simps =
 
 ML {*
 val [Network_Ask, Network_Giv, Network_Rel, Network_AllowedActs,
-     Network_preserves_allocGiv, Network_preserves_rel, 
-     Network_preserves_ask]  =  
-        thm "Network" |> simplify (simpset() addsimps (thms "network_spec_simps"))
+     Network_preserves_allocGiv, Network_preserves_rel,
+     Network_preserves_ask]  =
+        @{thm Network} |> simplify (@{simpset} addsimps @{thms network_spec_simps})
                 |> list_of_Int;
 
 bind_thm ("Network_Ask", Network_Ask);
@@ -602,9 +591,9 @@ lemmas alloc_spec_simps =
 
 ML {*
 val [Alloc_Increasing_0, Alloc_Safety, Alloc_Progress, Alloc_AllowedActs,
-     Alloc_preserves_allocRel, Alloc_preserves_allocAsk, 
-     Alloc_preserves_dummy] = 
-        thm "Alloc" |> simplify (simpset() addsimps (thms "alloc_spec_simps")) 
+     Alloc_preserves_allocRel, Alloc_preserves_allocAsk,
+     Alloc_preserves_dummy] =
+        @{thm Alloc} |> simplify (@{simpset} addsimps @{thms alloc_spec_simps})
               |> list_of_Int;
 
 bind_thm ("Alloc_Increasing_0", Alloc_Increasing_0);
@@ -617,10 +606,8 @@ bind_thm ("Alloc_preserves_dummy", Alloc_preserves_dummy);
 *}
 
 text{*Strip off the INT in the guarantees postcondition*}
-ML
-{*
-bind_thm ("Alloc_Increasing", normalize Alloc_Increasing_0)
-*}
+
+lemmas Alloc_Increasing = Alloc_Increasing_0 [normalized]
 
 declare
   Alloc_preserves_allocRel [iff]
@@ -630,20 +617,20 @@ declare
 
 subsection{*Components Lemmas [MUST BE AUTOMATED]*}
 
-lemma Network_component_System: "Network Join  
-      ((rename sysOfClient  
-        (plam x: (lessThan Nclients). rename client_map Client)) Join  
-       rename sysOfAlloc Alloc)  
+lemma Network_component_System: "Network Join
+      ((rename sysOfClient
+        (plam x: (lessThan Nclients). rename client_map Client)) Join
+       rename sysOfAlloc Alloc)
       = System"
   by (simp add: System_def Join_ac)
 
-lemma Client_component_System: "(rename sysOfClient  
-       (plam x: (lessThan Nclients). rename client_map Client)) Join  
+lemma Client_component_System: "(rename sysOfClient
+       (plam x: (lessThan Nclients). rename client_map Client)) Join
       (Network Join rename sysOfAlloc Alloc)  =  System"
   by (simp add: System_def Join_ac)
 
-lemma Alloc_component_System: "rename sysOfAlloc Alloc Join  
-       ((rename sysOfClient (plam x: (lessThan Nclients). rename client_map Client)) Join  
+lemma Alloc_component_System: "rename sysOfAlloc Alloc Join
+       ((rename sysOfClient (plam x: (lessThan Nclients). rename client_map Client)) Join
         Network)  =  System"
   by (simp add: System_def Join_ac)
 
@@ -658,8 +645,8 @@ text{** These preservation laws should be generated automatically **}
 lemma Client_Allowed [simp]: "Allowed Client = preserves rel Int preserves ask"
   by (auto simp add: Allowed_def Client_AllowedActs safety_prop_Acts_iff)
 
-lemma Network_Allowed [simp]: "Allowed Network =         
-        preserves allocRel Int  
+lemma Network_Allowed [simp]: "Allowed Network =
+        preserves allocRel Int
         (INT i: lessThan Nclients. preserves(giv o sub i o client))"
   by (auto simp add: Allowed_def Network_AllowedActs safety_prop_Acts_iff)
 
@@ -677,14 +664,14 @@ lemma OK_lift_rename_Client [simp]: "OK I (%i. lift i (rename client_map Client)
 
 lemma fst_lift_map_eq_fst [simp]: "fst (lift_map i x) i = fst x"
 apply (insert fst_o_lift_map [of i])
-apply (drule fun_cong [where x=x])  
+apply (drule fun_cong [where x=x])
 apply (simp add: o_def);
 done
 
 lemma fst_o_lift_map' [simp]:
      "(f \<circ> sub i \<circ> fst \<circ> lift_map i \<circ> g) = f o fst o g"
-apply (subst fst_o_lift_map [symmetric]) 
-apply (simp only: o_assoc) 
+apply (subst fst_o_lift_map [symmetric])
+apply (simp only: o_assoc)
 done
 
 
@@ -697,8 +684,8 @@ done
   RS (lift_lift_guarantees_eq RS iffD2)
   RS guarantees_PLam_I
   RS (bij_sysOfClient RS rename_rename_guarantees_eq RS iffD2)
-  |> simplify (simpset() addsimps [lift_image_eq_rename, o_def, split_def, 
-				   surj_rename RS surj_range])
+  |> simplify (simpset() addsimps [lift_image_eq_rename, o_def, split_def,
+                                   surj_rename RS surj_range])
 
 However, the "preserves" property remains to be discharged, and the unfolding
 of "o" and "sub" complicates subsequent reasoning.
@@ -708,41 +695,46 @@ ad-hoc!
 *)
 ML
 {*
-val rename_client_map_tac =
+fun rename_client_map_tac ss =
   EVERY [
-    simp_tac (simpset() addsimps [thm "rename_guarantees_eq_rename_inv"]) 1,
-    rtac (thm "guarantees_PLam_I") 1,
+    simp_tac (ss addsimps [thm "rename_guarantees_eq_rename_inv"]) 1,
+    rtac @{thm guarantees_PLam_I} 1,
     assume_tac 2,
-	 (*preserves: routine reasoning*)
-    asm_simp_tac (simpset() addsimps [thm "lift_preserves_sub"]) 2,
-	 (*the guarantee for  "lift i (rename client_map Client)" *)
+         (*preserves: routine reasoning*)
+    asm_simp_tac (ss addsimps [@{thm lift_preserves_sub}]) 2,
+         (*the guarantee for  "lift i (rename client_map Client)" *)
     asm_simp_tac
-	(simpset() addsimps [thm "lift_guarantees_eq_lift_inv",
-			     thm "rename_guarantees_eq_rename_inv",
-			     thm "bij_imp_bij_inv", thm "surj_rename" RS thm "surj_range",
-			     thm "inv_inv_eq"]) 1,
+        (ss addsimps [@{thm lift_guarantees_eq_lift_inv},
+                      @{thm rename_guarantees_eq_rename_inv},
+                      @{thm bij_imp_bij_inv}, @{thm surj_rename} RS @{thm surj_range},
+                      @{thm inv_inv_eq}]) 1,
     asm_simp_tac
-        (simpset() addsimps [thm "o_def", thm "non_dummy_def", thm "guarantees_Int_right"]) 1]
+        (@{simpset} addsimps [@{thm o_def}, @{thm non_dummy_def}, @{thm guarantees_Int_right}]) 1]
 *}
 
-text{*Lifting @{text Client_Increasing} to @{term systemState}*}
-lemma rename_Client_Increasing: "i : I  
-      ==> rename sysOfClient (plam x: I. rename client_map Client) :  
-            UNIV  guarantees   
-            Increasing (ask o sub i o client) Int  
-            Increasing (rel o sub i o client)"
-  by (tactic rename_client_map_tac)
+method_setup rename_client_map = {*
+  Method.ctxt_args (fn ctxt =>
+    Method.SIMPLE_METHOD (rename_client_map_tac (local_simpset_of ctxt)))
+*} ""
 
-lemma preserves_sub_fst_lift_map: "[| F : preserves w; i ~= j |]  
+text{*Lifting @{text Client_Increasing} to @{term systemState}*}
+lemma rename_Client_Increasing: "i : I
+      ==> rename sysOfClient (plam x: I. rename client_map Client) :
+            UNIV  guarantees
+            Increasing (ask o sub i o client) Int
+            Increasing (rel o sub i o client)"
+  by rename_client_map
+
+lemma preserves_sub_fst_lift_map: "[| F : preserves w; i ~= j |]
       ==> F : preserves (sub i o fst o lift_map j o funPair v w)"
   apply (auto simp add: lift_map_def split_def linorder_neq_iff o_def)
   apply (drule_tac [!] subset_preserves_o [THEN [2] rev_subsetD])
   apply (auto simp add: o_def)
   done
 
-lemma client_preserves_giv_oo_client_map: "[| i < Nclients; j < Nclients |]  
+lemma client_preserves_giv_oo_client_map: "[| i < Nclients; j < Nclients |]
       ==> Client : preserves (giv o sub i o fst o lift_map j o client_map)"
-  apply (case_tac "i=j") 
+  apply (case_tac "i=j")
   apply (simp, simp add: o_def non_dummy_def)
   apply (drule Client_preserves_dummy [THEN preserves_sub_fst_lift_map])
   apply (drule_tac [!] subset_preserves_o [THEN [2] rev_subsetD])
@@ -750,12 +742,12 @@ lemma client_preserves_giv_oo_client_map: "[| i < Nclients; j < Nclients |]
   done
 
 lemma rename_sysOfClient_ok_Network:
-  "rename sysOfClient (plam x: lessThan Nclients. rename client_map Client) 
+  "rename sysOfClient (plam x: lessThan Nclients. rename client_map Client)
     ok Network"
   by (auto simp add: ok_iff_Allowed client_preserves_giv_oo_client_map)
 
 lemma rename_sysOfClient_ok_Alloc:
-  "rename sysOfClient (plam x: lessThan Nclients. rename client_map Client) 
+  "rename sysOfClient (plam x: lessThan Nclients. rename client_map Client)
     ok rename sysOfAlloc Alloc"
   by (simp add: ok_iff_Allowed)
 
@@ -767,7 +759,7 @@ declare
   rename_sysOfClient_ok_Alloc [iff]
   rename_sysOfAlloc_ok_Network [iff]
 
-text{*The "ok" laws, re-oriented. 
+text{*The "ok" laws, re-oriented.
   But not sure this works: theorem @{text ok_commute} is needed below*}
 declare
   rename_sysOfClient_ok_Network [THEN ok_sym, iff]
@@ -775,7 +767,7 @@ declare
   rename_sysOfAlloc_ok_Network [THEN ok_sym]
 
 lemma System_Increasing: "i < Nclients
-      ==> System : Increasing (ask o sub i o client) Int  
+      ==> System : Increasing (ask o sub i o client) Int
                    Increasing (rel o sub i o client)"
   apply (rule component_guaranteesD [OF rename_Client_Increasing Client_component_System])
   apply auto
@@ -788,12 +780,12 @@ lemmas rename_guarantees_sysOfAlloc_I =
 (*Lifting Alloc_Increasing up to the level of systemState*)
 lemmas rename_Alloc_Increasing =
   Alloc_Increasing
-    [THEN rename_guarantees_sysOfAlloc_I, 
-     simplified surj_rename [THEN surj_range] o_def sub_apply 
-                rename_image_Increasing bij_sysOfAlloc 
+    [THEN rename_guarantees_sysOfAlloc_I,
+     simplified surj_rename [THEN surj_range] o_def sub_apply
+                rename_image_Increasing bij_sysOfAlloc
                 allocGiv_o_inv_sysOfAlloc_eq'];
 
-lemma System_Increasing_allocGiv: 
+lemma System_Increasing_allocGiv:
      "i < Nclients ==> System : Increasing (sub i o allocGiv)"
   apply (unfold System_def)
   apply (simp add: o_def)
@@ -812,19 +804,19 @@ text{* Follows consequences.
     The "Always (INT ...) formulation expresses the general safety property
     and allows it to be combined using @{text Always_Int_rule} below. *}
 
-lemma System_Follows_rel: 
+lemma System_Follows_rel:
   "i < Nclients ==> System : ((sub i o allocRel) Fols (rel o sub i o client))"
   apply (auto intro!: Network_Rel [THEN component_guaranteesD])
-  apply (simp add: ok_commute [of Network]) 
+  apply (simp add: ok_commute [of Network])
   done
 
-lemma System_Follows_ask: 
+lemma System_Follows_ask:
   "i < Nclients ==> System : ((sub i o allocAsk) Fols (ask o sub i o client))"
   apply (auto intro!: Network_Ask [THEN component_guaranteesD])
-  apply (simp add: ok_commute [of Network]) 
+  apply (simp add: ok_commute [of Network])
   done
 
-lemma System_Follows_allocGiv: 
+lemma System_Follows_allocGiv:
   "i < Nclients ==> System : (giv o sub i o client) Fols (sub i o allocGiv)"
   apply (auto intro!: Network_Giv [THEN component_guaranteesD]
     rename_Alloc_Increasing [THEN component_guaranteesD])
@@ -833,21 +825,21 @@ lemma System_Follows_allocGiv:
   done
 
 
-lemma Always_giv_le_allocGiv: "System : Always (INT i: lessThan Nclients.  
+lemma Always_giv_le_allocGiv: "System : Always (INT i: lessThan Nclients.
                        {s. (giv o sub i o client) s \<le> (sub i o allocGiv) s})"
   apply auto
   apply (erule System_Follows_allocGiv [THEN Follows_Bounded])
   done
 
 
-lemma Always_allocAsk_le_ask: "System : Always (INT i: lessThan Nclients.  
+lemma Always_allocAsk_le_ask: "System : Always (INT i: lessThan Nclients.
                        {s. (sub i o allocAsk) s \<le> (ask o sub i o client) s})"
   apply auto
   apply (erule System_Follows_ask [THEN Follows_Bounded])
   done
 
 
-lemma Always_allocRel_le_rel: "System : Always (INT i: lessThan Nclients.  
+lemma Always_allocRel_le_rel: "System : Always (INT i: lessThan Nclients.
                        {s. (sub i o allocRel) s \<le> (rel o sub i o client) s})"
   by (auto intro!: Follows_Bounded System_Follows_rel)
 
@@ -865,27 +857,27 @@ lemmas System_Increasing_allocRel = System_Follows_rel [THEN Follows_Increasing1
   gets rid of the other "o"s too.*)
 
 text{*safety (1), step 3*}
-lemma System_sum_bounded: 
+lemma System_sum_bounded:
     "System : Always {s. (\<Sum>i \<in> lessThan Nclients. (tokens o sub i o allocGiv) s)
             \<le> NbT + (\<Sum>i \<in> lessThan Nclients. (tokens o sub i o allocRel) s)}"
   apply (simp add: o_apply)
-  apply (insert Alloc_Safety [THEN rename_guarantees_sysOfAlloc_I])   
-  apply (simp add: o_def); 
-  apply (erule component_guaranteesD) 
+  apply (insert Alloc_Safety [THEN rename_guarantees_sysOfAlloc_I])
+  apply (simp add: o_def);
+  apply (erule component_guaranteesD)
   apply (auto simp add: System_Increasing_allocRel [simplified sub_apply o_def])
   done
 
 text{* Follows reasoning*}
 
-lemma Always_tokens_giv_le_allocGiv: "System : Always (INT i: lessThan Nclients.  
-                          {s. (tokens o giv o sub i o client) s  
+lemma Always_tokens_giv_le_allocGiv: "System : Always (INT i: lessThan Nclients.
+                          {s. (tokens o giv o sub i o client) s
                            \<le> (tokens o sub i o allocGiv) s})"
   apply (rule Always_giv_le_allocGiv [THEN Always_weaken])
   apply (auto intro: tokens_mono_prefix simp add: o_apply)
   done
 
-lemma Always_tokens_allocRel_le_rel: "System : Always (INT i: lessThan Nclients.  
-                          {s. (tokens o sub i o allocRel) s  
+lemma Always_tokens_allocRel_le_rel: "System : Always (INT i: lessThan Nclients.
+                          {s. (tokens o sub i o allocRel) s
                            \<le> (tokens o rel o sub i o client) s})"
   apply (rule Always_allocRel_le_rel [THEN Always_weaken])
   apply (auto intro: tokens_mono_prefix simp add: o_apply)
@@ -915,15 +907,15 @@ text{*progress (2), step 2; see also @{text System_Increasing_allocRel}*}
 lemmas System_Increasing_allocAsk =  System_Follows_ask [THEN Follows_Increasing1, standard]
 
 text{*progress (2), step 3: lifting @{text Client_Bounded} to systemState*}
-lemma rename_Client_Bounded: "i : I  
-    ==> rename sysOfClient (plam x: I. rename client_map Client) :  
-          UNIV  guarantees   
+lemma rename_Client_Bounded: "i : I
+    ==> rename sysOfClient (plam x: I. rename client_map Client) :
+          UNIV  guarantees
           Always {s. ALL elt : set ((ask o sub i o client) s). elt \<le> NbT}"
-  by (tactic rename_client_map_tac)
+  by rename_client_map
 
 
-lemma System_Bounded_ask: "i < Nclients  
-      ==> System : Always  
+lemma System_Bounded_ask: "i < Nclients
+      ==> System : Always
                     {s. ALL elt : set ((ask o sub i o client) s). elt \<le> NbT}"
   apply (rule component_guaranteesD [OF rename_Client_Bounded Client_component_System])
   apply auto
@@ -934,7 +926,7 @@ lemma Collect_all_imp_eq: "{x. ALL y. P y --> Q x y} = (INT y: {y. P y}. {x. Q x
   done
 
 text{*progress (2), step 4*}
-lemma System_Bounded_allocAsk: "System : Always {s. ALL i<Nclients.  
+lemma System_Bounded_allocAsk: "System : Always {s. ALL i<Nclients.
                           ALL elt : set ((sub i o allocAsk) s). elt \<le> NbT}"
   apply (auto simp add: Collect_all_imp_eq)
   apply (tactic {* rtac (Always_Int_rule [thm "Always_allocAsk_le_ask",
@@ -949,23 +941,23 @@ text{*progress (2), step 6*}
 lemmas System_Increasing_giv =  System_Follows_allocGiv [THEN Follows_Increasing1, standard]
 
 
-lemma rename_Client_Progress: "i: I  
-   ==> rename sysOfClient (plam x: I. rename client_map Client)  
-        : Increasing (giv o sub i o client)   
-          guarantees  
-          (INT h. {s. h \<le> (giv o sub i o client) s &  
-                            h pfixGe (ask o sub i o client) s}   
+lemma rename_Client_Progress: "i: I
+   ==> rename sysOfClient (plam x: I. rename client_map Client)
+        : Increasing (giv o sub i o client)
+          guarantees
+          (INT h. {s. h \<le> (giv o sub i o client) s &
+                            h pfixGe (ask o sub i o client) s}
                   LeadsTo {s. tokens h \<le> (tokens o rel o sub i o client) s})"
-  apply (tactic rename_client_map_tac)
+  apply rename_client_map
   apply (simp add: Client_Progress [simplified o_def])
   done
 
 
 text{*progress (2), step 7*}
-lemma System_Client_Progress: 
-  "System : (INT i : (lessThan Nclients).  
-            INT h. {s. h \<le> (giv o sub i o client) s &  
-                       h pfixGe (ask o sub i o client) s}   
+lemma System_Client_Progress:
+  "System : (INT i : (lessThan Nclients).
+            INT h. {s. h \<le> (giv o sub i o client) s &
+                       h pfixGe (ask o sub i o client) s}
                 LeadsTo {s. tokens h \<le> (tokens o rel o sub i o client) s})"
   apply (rule INT_I)
 (*Couldn't have just used Auto_tac since the "INT h" must be kept*)
@@ -974,7 +966,7 @@ lemma System_Client_Progress:
   done
 
 (*Concludes
- System : {s. k \<le> (sub i o allocGiv) s} 
+ System : {s. k \<le> (sub i o allocGiv) s}
           LeadsTo
           {s. (sub i o allocAsk) s \<le> (ask o sub i o client) s} Int
           {s. k \<le> (giv o sub i o client) s} *)
@@ -985,17 +977,17 @@ lemmas System_lemma1 =
 
 lemmas System_lemma2 =
   PSP_Stable [OF System_lemma1
-	      System_Follows_ask [THEN Follows_Increasing1, THEN IncreasingD]]
+              System_Follows_ask [THEN Follows_Increasing1, THEN IncreasingD]]
 
 
-lemma System_lemma3: "i < Nclients  
-      ==> System : {s. h \<le> (sub i o allocGiv) s &       
-                       h pfixGe (sub i o allocAsk) s}    
-                   LeadsTo   
-                   {s. h \<le> (giv o sub i o client) s &   
+lemma System_lemma3: "i < Nclients
+      ==> System : {s. h \<le> (sub i o allocGiv) s &
+                       h pfixGe (sub i o allocAsk) s}
+                   LeadsTo
+                   {s. h \<le> (giv o sub i o client) s &
                        h pfixGe (ask o sub i o client) s}"
   apply (rule single_LeadsTo_I)
-  apply (rule_tac k6 = "h" and x2 = " (sub i o allocAsk) s" 
+  apply (rule_tac k6 = "h" and x2 = " (sub i o allocAsk) s"
          in System_lemma2 [THEN LeadsTo_weaken])
   apply auto
   apply (blast intro: trans_Ge [THEN trans_genPrefix, THEN transD] prefix_imp_pfixGe)
@@ -1003,9 +995,9 @@ lemma System_lemma3: "i < Nclients
 
 
 text{*progress (2), step 8: Client i's "release" action is visible system-wide*}
-lemma System_Alloc_Client_Progress: "i < Nclients   
-      ==> System : {s. h \<le> (sub i o allocGiv) s &  
-                       h pfixGe (sub i o allocAsk) s}   
+lemma System_Alloc_Client_Progress: "i < Nclients
+      ==> System : {s. h \<le> (sub i o allocGiv) s &
+                       h pfixGe (sub i o allocAsk) s}
                    LeadsTo {s. tokens h \<le> (tokens o sub i o allocRel) s}"
   apply (rule LeadsTo_Trans)
    prefer 2
@@ -1023,15 +1015,15 @@ lemma System_Alloc_Client_Progress: "i < Nclients
 text{*Lifting @{text Alloc_Progress} up to the level of systemState*}
 
 text{*progress (2), step 9*}
-lemma System_Alloc_Progress: 
- "System : (INT i : (lessThan Nclients).  
-            INT h. {s. h \<le> (sub i o allocAsk) s}   
+lemma System_Alloc_Progress:
+ "System : (INT i : (lessThan Nclients).
+            INT h. {s. h \<le> (sub i o allocAsk) s}
                    LeadsTo {s. h pfixLe (sub i o allocGiv) s})"
   apply (simp only: o_apply sub_def)
-  apply (insert Alloc_Progress [THEN rename_guarantees_sysOfAlloc_I]) 
-  apply (simp add: o_def del: Set.INT_iff); 
+  apply (insert Alloc_Progress [THEN rename_guarantees_sysOfAlloc_I])
+  apply (simp add: o_def del: Set.INT_iff);
   apply (erule component_guaranteesD)
-  apply (auto simp add: 
+  apply (auto simp add:
     System_Increasing_allocRel [simplified sub_apply o_def]
     System_Increasing_allocAsk [simplified sub_apply o_def]
     System_Bounded_allocAsk [simplified sub_apply o_def]
@@ -1056,13 +1048,13 @@ theorem System_correct: "System : system_spec"
 
 text{* Some obsolete lemmas *}
 
-lemma non_dummy_eq_o_funPair: "non_dummy = (% (g,a,r). (| giv = g, ask = a, rel = r |)) o  
+lemma non_dummy_eq_o_funPair: "non_dummy = (% (g,a,r). (| giv = g, ask = a, rel = r |)) o
                               (funPair giv (funPair ask rel))"
   apply (rule ext)
   apply (auto simp add: o_def non_dummy_def)
   done
 
-lemma preserves_non_dummy_eq: "(preserves non_dummy) =  
+lemma preserves_non_dummy_eq: "(preserves non_dummy) =
       (preserves rel Int preserves ask Int preserves giv)"
   apply (simp add: non_dummy_eq_o_funPair)
   apply auto
